feat: merged Brandon's work from the 'dev' branch into new project structure

Proofs/Main_Proof.v
@@ -10,7 +10,7 @@
    4. Only prove correctness for valid inputs (caller's responsibility to provide valid input)
 *)
 
-Require Import Picinae_armv8_pcode.
+(* Import standard libraries *)
 Require Import Utf8.
 Require Import NArith.
 Require Import ZArith.
@@ -27,7 +27,207 @@ Require Import BitWidth.
 Require Import Specification.
 Require Import Invariants.
 
+(* Import Picinae notations/tactics *)
+Require Import Picinae_armv8_pcode.
 Import ARM8Notations.
 
 Open Scope N.
 
+(* ARMv8 lifter creates non-writeable code *)
+Theorem atoi_nwc:
+  forall s1 s2, atoi_lo_atoi_armv8 s1 = atoi_lo_atoi_armv8 s2.
+Proof.
+  reflexivity.
+Qed.
+
+(* ARMv8 lifter produces well-typed IL *)
+Theorem atoi_welltyped: 
+  welltyped_prog arm8typctx atoi_lo_atoi_armv8.
+Proof. 
+  Picinae_typecheck. 
+Qed.
+
+(* Post condition point for atoi *)
+Definition atoi_exit (t:trace) : bool :=
+  match t with 
+  | (Addr 0x100070,_)::_ => true
+  | _ => false 
+  end.
+
+(* ========== Correctness Theorems ========== *)
+
+Ltac step := time arm8_step; try exact I.
+
+(* A single byte will never have a value greater than 2^32. *)
+Lemma mod_too_big_to_matter:
+  forall p m, m Ⓑ[ p ] mod 2 ^ 32 = m Ⓑ[ p ].
+Proof.
+  intros. apply getmem_mod with (w:=64) (e:=LittleE) (n2:=4) (n1:=1) (m:=m) (a:=p).
+Qed.
+
+Theorem atoi_partial_correctness:
+  forall s t s' x' mem p 
+    (PRE: atoi_pre p s t x' s')
+    (MEM: s V_MEM64 = mem),
+  satisfies_all atoi_lo_atoi_armv8 (atoi_invs mem p) atoi_exit ((x',s')::t).
+Proof.
+  intros. destruct PRE as (ENTRY & MDL & RX1). unfold inv_entry in RX1. apply prove_invs.
+
+  (* Base Case: Entry, 1048576 *)
+  Print inv_entry.
+  simpl. rewrite ENTRY. step. assumption.
+
+  (* Set up the inductive case *)
+  intros. erewrite startof_prefix in ENTRY; try eassumption.
+  eapply models_at_invariant; try eassumption. apply atoi_welltyped. intro MDL1.
+  clear - PRE MDL1.
+  destruct_inv 64 PRE.
+
+  (* 1048576 -> 1048580, start of whitespace loop *)
+  (* Prove that we have either skipped over j bytes of whitespace where j < i, or i = 0. *)
+  step. unfold inv_whitespace_loop. unfold all_whitespace_until. exists 0. split.
+    right; reflexivity.
+    psimpl; reflexivity.
+
+  (* 1048580 -> 1048636 and 1048580 -> 1048600 *)
+  destruct PRE as (i & H0 & H1). unfold all_whitespace_until in H0. destruct H0.
+    (* 1048580 -> 1048636: Prove that the current character is whitespace. *)
+    admit.
+    (* 1048580 -> 1048600: Prove that the current character is NOT whitespace, 
+    and that there exists j whitespace bytes *)
+    admit.
+
+  (* 1048600 -> 1048620 and 1048600 -> 1048624 *)
+  unfold inv_after_whitespace, first_nonwhitespace, all_whitespace_until in PRE.
+  step. step.
+    (* BC: Character is a plus sign, so we know a sign exists. *)
+    step. step. intros. specialize PRE with (i:=i). 
+    destruct PRE as (WS & REG); destruct WS as (NUMWS & NONWS); destruct REG as (X0 & X1).
+    unfold inv_sign_exists. exists (i+1). split. right. split.
+      (* The current character is in fact a plus sign *)
+      apply Neqb_ok in BC. rewrite X0 in BC. rewrite mod_too_big_to_matter in BC. assumption.
+      (* R_X3 is equal to 0 because this is a plus sign (positive number). *)
+      psimpl; reflexivity.
+      (* We know at what index the digits should start. *)
+      unfold digit_start, first_nonwhitespace, all_whitespace_until. repeat split; try assumption.
+      left. split.
+        unfold sign_indicator_exists. right. split.
+          apply Neqb_ok in BC. rewrite X0 in BC. rewrite mod_too_big_to_matter in BC. assumption.
+          psimpl. reflexivity.
+        reflexivity.
+    (* BC: Character is NOT a plus sign *)
+    step. step.
+      (* BC0: Character is a minus sign *)
+      step. intros. specialize PRE with (i:=i). 
+      destruct PRE as (WS & REG); destruct WS as (NUMWS & NONWS); destruct REG as (X0 & X1).
+      unfold inv_sign_exists. unfold sign_indicator_exists. exists (i+1). split. left. split.
+        (* The current character is in fact a minus sign *)
+        apply Neqb_ok in BC0. rewrite X0 in BC0. rewrite mod_too_big_to_matter in BC0. assumption.
+        (* The current character is in fact a minus sign *)
+        psimpl; reflexivity.
+        (* We know at what index the digits should start. *)
+        unfold digit_start. split. unfold first_nonwhitespace, all_whitespace_until. left. split.
+          unfold sign_indicator_exists. left. split.
+            apply Neqb_ok in BC0. rewrite X0 in BC0. rewrite mod_too_big_to_matter in BC0. assumption.
+            psimpl; reflexivity.
+          reflexivity.
+        psimpl; assumption.
+      (* BC0: Character is NOT a minus sign *)
+      step. step. intros. specialize PRE with (i:=i). 
+      destruct PRE as (WS & REG); destruct WS as (NUMWS & NONWS); destruct REG as (X0 & X1). exists i.
+      unfold inv_post_sign. (* At this point, there is no sign indicator. *) split. right. split.
+        (* There is no sign indicator. *)
+        unfold sign_indicator_exists.
+        apply N.eqb_neq in BC. rewrite X0 in BC. rewrite mod_too_big_to_matter in BC.
+        apply N.eqb_neq in BC0. rewrite X0 in BC0. rewrite mod_too_big_to_matter in BC0.
+        psimpl. psimpl in BC. psimpl in BC0. tauto. (* trust me bro *)
+        (* R_X3 = 0 because there is no sign indicator. *)
+        psimpl; reflexivity.
+        (* We know at what index the digits should start. *)
+        unfold digit_start. split.
+          unfold sign_indicator_exists. right. split.
+            apply N.eqb_neq in BC. rewrite X0 in BC. rewrite mod_too_big_to_matter in BC.
+            apply N.eqb_neq in BC0. rewrite X0 in BC0. rewrite mod_too_big_to_matter in BC0.
+            psimpl. psimpl in BC. psimpl in BC0. tauto.
+          reflexivity.
+        psimpl; assumption.
+
+  (* 1048620 -> 1048624: There is a sign indicator. *)
+  step. intros. 
+  (* Precondition unfolding *)
+  specialize PRE with (i:=i). destruct PRE. rename x into j; exists j. 
+  unfold inv_sign_exists in H. destruct H as (SIGN & DIGIT). destruct DIGIT as (DIGIT & X1).
+  (* Goal unfolding *)
+  unfold inv_post_sign, inv_sign_exists.
+  (* The Proof *)
+  split. 
+    (* There is a sign indicator and we know R_X3 is 0 or 1. *)
+    left. split.
+      (* There is a sign indicator. *)
+      unfold sign_indicator_exists in *. destruct SIGN as [SIGN|].
+        (* The sign was a minus sign. *)
+        destruct SIGN as (SIGN & X3). left; split; assumption.
+        (* The sign was a plus sign. *)
+        destruct H as (SIGN & X3). right; split; assumption.
+      (* R_X3 is either 0 or 1. *)
+      psimpl. destruct SIGN. 
+        destruct H. right; assumption.
+        destruct H. left; assumption.
+    (* We know the index of digit start. *)
+    destruct DIGIT.
+      (* A sign indicator exists; the index of digit start is just after this sign indicator. *)
+      split.
+        unfold digit_start. left. split.
+          unfold sign_indicator_exists in *. psimpl. psimpl in SIGN. assumption.
+          destruct H. assumption.
+        psimpl. destruct H. subst. rewrite X1. psimpl; reflexivity.
+      (* A sign indicator does NOT exist. *)
+      destruct H. contradiction.
+
+  (* 1048624 -> 1048664 *)
+  step. step. step. intros. 
+  specialize PRE with (i:=i); unfold inv_post_sign, inv_sign_exists, sign_indicator_exists in PRE.
+  psimpl in PRE. destruct PRE; destruct H as (PRE & DSTART). rename x into j. destruct DSTART as (DSTART & X1).
+  destruct PRE.
+  (* Sign indicator exists. *)
+  exists j, 0, 0. unfold inv_digit_loop. split.
+    (* We know inv_post_sign still holds despite R_X0 and R_X4 being changed. *)
+    unfold inv_post_sign. split. 
+      unfold sign_indicator_exists. psimpl. left. assumption.
+      split; assumption.
+    (* We have seen k=0 valid digits so far. *)
+    split.
+      unfold all_digits. intros. apply N.nlt_0_r in H0. exfalso; assumption.
+    split.
+      apply N.le_refl.
+      psimpl. split.
+        assumption.
+        reflexivity.
+  (* Sign indicator does not exist. *)
+  exists j, 0, 0. unfold inv_digit_loop. split.
+    (* We know inv_post_sign still holds despite R_X0 and R_X4 being changed. *)
+    unfold inv_post_sign. split. 
+      unfold inv_sign_exists, sign_indicator_exists. psimpl. right. assumption. 
+      split; assumption.
+    (* We have seen k=0 valid digits so far. *)
+    split.
+      unfold all_digits. intros. apply N.nlt_0_r in H0. exfalso; assumption.
+    split.
+      apply N.le_refl.
+      psimpl. split.
+        assumption. 
+        reflexivity.
+
+  (* 1048636 -> 1048580 - From inside whitespace loop back to the start of it*)
+  step. step. 
+  specialize PRE with (i:=0). destruct PRE; psimpl in H. destruct H0.
+  unfold inv_whitespace_loop, all_whitespace_until. exists 1. split.
+    left. psimpl; assumption.
+    psimpl. rewrite H1. psimpl; reflexivity.
+
+  (* 1048652 -> 1048664 *)
+  step. step. step. admit.
+
+  (* 1048664 -> 1048652 and 1048664 -> EXIT *)
+  admit.
+Admitted.
